showed cont recvTSPF

CaseStudies/ABP/ABP_TSPS.thy
@@ -10,13 +10,13 @@ theory ABP_TSPS
     
 begin
 
-  default_sort message 
+  default_sort countable
   
 (* ----------------------------------------------------------------------- *)
 section \<open>Datatype Definition\<close>
 (* ----------------------------------------------------------------------- *)
   
-datatype 'a::type MABP = BoolPair "('a * bool)" | Bool bool | Data 'a
+datatype 'a::countable MABP = BoolPair "('a * bool)" | Bool bool | Data 'a
 
 instantiation MABP ::  (countable) countable
 begin
@@ -33,12 +33,14 @@ fun ctype_MABP :: "channel \<Rightarrow> 'a MABP set" where
   "ctype_MABP dr = range BoolPair" |
   "ctype_MABP as = range Bool" |
   "ctype_MABP ar = range Bool" |
-  "ctype_MABP other = {}"
+  "ctype_MABP other = undefined"
 
   instance ..
 end
 
-declare [[show_types]]  
+ declare [[show_types]]
+  declare [[show_sorts]]
+declare [[show_consts]]
   
 (* ----------------------------------------------------------------------- *)
 section \<open>Definitions\<close>
@@ -63,10 +65,8 @@ in (\<lambda> x. (tsbDom\<cdot>x = {dr}) \<leadsto> [ar    \<mapsto> tsMap Bool\
 
 subsection \<open>receiver\<close> 
 definition recvTSPF :: "'a MABP TSPF" where
-"recvTSPF \<equiv> 
-let recRes = (\<lambda> x. tsRec\<cdot>((tsMap invBoolPair)\<cdot>(x . dr)))
-in Abs_CTSPF (\<lambda> x. (tsbDom\<cdot>x = {dr}) \<leadsto> [ar    \<mapsto> tsMap Bool\<cdot>(fst (recRes x)),
-                                        abpOut \<mapsto> tsMap Data\<cdot>(snd (recRes x))]\<Omega>)"
+"recvTSPF \<equiv> Abs_CTSPF (\<lambda> x. (tsbDom\<cdot>x = {dr}) \<leadsto> [ar    \<mapsto> (tsMap::(bool \<Rightarrow> 'a MABP) \<Rightarrow> bool tstream \<rightarrow> 'a MABP tstream) Bool\<cdot>(fst ( tsRec\<cdot>((tsMap invBoolPair)\<cdot>(x . dr)))),
+                                        abpOut \<mapsto> (tsMap::('a \<Rightarrow> 'a MABP) \<Rightarrow> 'a tstream \<rightarrow> 'a MABP tstream) Data\<cdot>(snd ( tsRec\<cdot>((tsMap invBoolPair)\<cdot>(x . dr))))]\<Omega>)"
 
 subsection \<open>medium_rs\<close>
   (* medium from receiver to sender *)
@@ -112,50 +112,55 @@ lemma data_data_inv [simp]: "(inv Data) (Data x) = x"
 
 subsection \<open>receiver\<close>
 
-lemma "cont (\<lambda> x. tsMap Bool\<cdot>(fst (tsRec\<cdot>((tsMap invBoolPair)\<cdot>(x .dr)))))"
-  by (simp add: monofun_fst)
+subsection \<open>defs\<close>  
   
-lemma "x \<sqsubseteq> y \<Longrightarrow> tsMap Bool\<cdot>(fst (tsRec\<cdot>(tsMap invBoolPair\<cdot>(x  .  dr)))) \<sqsubseteq> tsMap Bool\<cdot>(fst (tsRec\<cdot>(tsMap invBoolPair\<cdot>(y  .  dr))))"
-  by (simp add: fst_monofun monofun_cfun_arg tsbgetch_below)
-
-definition testf :: "'a MABP TSB \<Rightarrow> 'a MABP tstream"  where
-  "testf \<equiv> (\<lambda> x. tsMap Bool\<cdot>(fst (tsRec\<cdot>((tsMap invBoolPair)\<cdot>(x .dr)))))"
+      (* helper functions to prove cont *)
+definition recvCH1 :: "'a MABP TSB \<Rightarrow> 'a MABP tstream"  where
+"recvCH1 \<equiv> (\<lambda> x. tsMap Bool\<cdot>(fst (tsRec\<cdot>((tsMap invBoolPair)\<cdot>(x .dr)))))"
     
-lemma f21: assumes "  chain Y" and "tsbDom\<cdot>(\<Squnion>i::nat. Y i) = {dr}"
-  shows "testf ((\<Squnion>i. Y i)) = (\<Squnion>i. (testf ((Y i))))"
+definition recvCH2 :: "'a MABP TSB \<Rightarrow> 'a MABP tstream"  where
+"recvCH2 \<equiv> (\<lambda> x. tsMap Data\<cdot>(snd (tsRec\<cdot>((tsMap invBoolPair)\<cdot>(x .dr)))))"
+  
+lemma recvCH1_contlub: assumes "  chain Y" and "tsbDom\<cdot>(\<Squnion>i::nat. Y i) = {dr}"
+  shows "recvCH1 ((\<Squnion>i. Y i)) = (\<Squnion>i. (recvCH1 ((Y i))))"
   apply (rule cont2contlubE)
-  by (simp_all add: assms testf_def)
+  by (simp_all add: assms recvCH1_def)
+    
+lemma recvCH2_contlub: assumes "  chain Y" and "tsbDom\<cdot>(\<Squnion>i::nat. Y i) = {dr}"
+  shows "recvCH2 ((\<Squnion>i. Y i)) = (\<Squnion>i. (recvCH2 ((Y i))))"
+  apply (rule cont2contlubE)
+  by (simp_all add: assms recvCH2_def)
 
-lemma testme: "tsMap Bool\<cdot>(fst (tsRec\<cdot>((tsMap invBoolPair)\<cdot>(x .dr)))) = (testf::'a MABP TSB \<Rightarrow> 'a MABP tstream) x"
-  by (simp add: testf_def)
+    
+lemma to_recvch1: "tsMap Bool\<cdot>(fst (tsRec\<cdot>((tsMap invBoolPair)\<cdot>(x .dr)))) 
+                    = (recvCH1::'a MABP TSB \<Rightarrow> 'a MABP tstream) x"
+  by (simp add: recvCH1_def)
+    
+lemma to_recvch2: "tsMap Data\<cdot>(snd (tsRec\<cdot>((tsMap invBoolPair)\<cdot>(x .dr)))) 
+                    = (recvCH2::'a MABP TSB \<Rightarrow> 'a MABP tstream) x"
+  by (simp add: recvCH2_def)
   
-(*
-lemma assumes "  chain Y" and "tsbDom\<cdot>(\<Squnion>i::nat. Y i) = {dr}"
-  shows "tsMap Bool\<cdot>(fst (tsRec\<cdot>(tsMap invBoolPair\<cdot>((\<Squnion>i. Y i)  .  dr)))) \<sqsubseteq> (\<Squnion>i::nat. tsMap Bool\<cdot>(fst (tsRec\<cdot>(tsMap invBoolPair\<cdot>(Y i  .  dr)))))"
-proof -
-  have f1: "tsMap Bool\<cdot>(fst (tsRec\<cdot>(tsMap invBoolPair\<cdot>((\<Squnion>i. Y i)  .  dr)))) = testf ((\<Squnion>i. Y i)) "
-    by (simp add: testf_def)
-  have f2: "(\<Squnion>i::nat. tsMap Bool\<cdot>(fst (tsRec\<cdot>(tsMap invBoolPair\<cdot>(Y i  .  dr))))) = (\<Squnion>i. (testf ((Y i))))"
-    by (simp add: testf_def)
-  show ?thesis
-   apply (subst testme)
-      
- 
-  
-lemma "monofun (\<lambda> x.  tsMap Bool\<cdot>(fst (tsRec\<cdot>(x))))" 
-  apply (rule monofunI)
-    oops
-*)
+   
+
+
+lemma fixes Y :: "nat \<Rightarrow> 'a MABP TSB" assumes "chain Y" and "tsbDom\<cdot>(\<Squnion>i::nat. Y i) = {dr}"
+  shows "(tsMap::(bool \<Rightarrow> 'a MABP) \<Rightarrow> bool tstream \<rightarrow> 'a MABP tstream) 
+          Bool\<cdot>(fst ((tsRec)\<cdot>(tsMap invBoolPair\<cdot>((\<Squnion>i. Y i)  .  dr)))) \<sqsubseteq> 
+          (\<Squnion>i::nat. tsMap Bool\<cdot>(fst ((tsRec)\<cdot>(tsMap invBoolPair\<cdot>(Y i  .  dr)))))"
+  by (metis (mono_tags, lifting) assms(1) assms(2) recvCH1_contlub lub_eq po_eq_conv recvCH1_def)
+    
+
     
 lemma recv_tsb_well [simp]:
   shows "tsb_well [ar \<mapsto> tsMap Bool\<cdot>(fst (tsRec\<cdot>((tsMap invBoolPair)\<cdot>(x . dr)))),
-                                    abpOut \<mapsto> tsMap Data\<cdot>(snd (tsRec\<cdot>((tsMap invBoolPair)\<cdot>(x . dr))))]"
+                                  abpOut \<mapsto> tsMap Data\<cdot>(snd (tsRec\<cdot>((tsMap invBoolPair)\<cdot>(x . dr))))]"
   apply (rule tsb_wellI)
   apply (simp add: tsmap_tsdom_range)
   by blast
     
-lemma recv_tsb_dom: "tsbDom\<cdot>( [ar \<mapsto> tsMap Bool\<cdot>(fst (tsRec\<cdot>((tsMap invBoolPair)\<cdot>(x . dr)))),
-                                    abpOut \<mapsto> tsMap Data\<cdot>(snd (tsRec\<cdot>((tsMap invBoolPair)\<cdot>(x . dr))))]\<Omega>) = {ar, abpOut}"
+lemma recv_tsb_dom: "tsbDom\<cdot>([ar \<mapsto> tsMap Bool\<cdot>(fst (tsRec\<cdot>((tsMap invBoolPair)\<cdot>(x . dr)))),
+                              abpOut \<mapsto> tsMap Data\<cdot>(snd (tsRec\<cdot>((tsMap invBoolPair)\<cdot>(x . dr))))]\<Omega>) 
+                     = {ar, abpOut}"
   apply (simp add: tsbdom_rep_eq)
     by auto
  
@@ -169,8 +174,9 @@ lemma rec_tsb_mono: "\<And>(x::'a MABP TSB) y::'a MABP TSB. tsbDom\<cdot>x = {dr
        by (simp add: fst_monofun snd_monofun monofun_cfun_arg tsbgetch_below)
      
   
-lemma recvTSPF_mono [simp]: "monofun (\<lambda> x. (tsbDom\<cdot>x = {dr}) \<leadsto> [ar \<mapsto> tsMap Bool\<cdot>(fst (tsRec\<cdot>((tsMap invBoolPair)\<cdot>(x . dr)))),
-                                        abpOut \<mapsto> tsMap Data\<cdot>(snd (tsRec\<cdot>((tsMap invBoolPair)\<cdot>(x . dr))))]\<Omega>)"
+lemma recvTSPF_mono [simp]: "monofun (\<lambda> x. (tsbDom\<cdot>x = {dr}) \<leadsto> 
+                                    [ar \<mapsto> tsMap Bool\<cdot>(fst (tsRec\<cdot>((tsMap invBoolPair)\<cdot>(x . dr)))),
+                                     abpOut \<mapsto> tsMap Data\<cdot>(snd (tsRec\<cdot>((tsMap invBoolPair)\<cdot>(x . dr))))]\<Omega>)"
   apply (rule tspf_monoI)
   apply (rule tsb_below)
    apply (simp_all add: tsbdom_below tsbdom_rep_eq tsbgetch_rep_eq)
@@ -187,20 +193,26 @@ lemma recvTSPF_tsb_getc: assumes "chain Y" and "tsbDom\<cdot>(\<Squnion>i. Y i) 
 proof (rule lubgetCh)
    have f2: "\<And> i. tsbDom\<cdot>(Y i) =  tsbDom\<cdot>(\<Squnion>i. Y i)"
      by (simp add: assms(1))
-   show tb_chain: "chain (\<lambda>i::nat. [ar \<mapsto> tsMap Bool\<cdot>(fst (tsRec\<cdot>(tsMap invBoolPair\<cdot>(Y i  .  dr)))), abpOut \<mapsto>
-                      tsMap Data\<cdot>(snd (tsRec\<cdot>(tsMap invBoolPair\<cdot>(Y i  .  dr))))]\<Omega>)"
+   show tb_chain: "chain (\<lambda>i::nat. [ar \<mapsto> tsMap Bool\<cdot>(fst (tsRec\<cdot>(tsMap invBoolPair\<cdot>(Y i  .  dr)))), 
+                             abpOut \<mapsto> tsMap Data\<cdot>(snd (tsRec\<cdot>(tsMap invBoolPair\<cdot>(Y i  .  dr))))]\<Omega>)"
      by (simp add: assms(1) assms(2) po_class.chainE po_class.chainI rec_tsb_mono)
    
-   show " c \<in> tsbDom\<cdot>(\<Squnion>i::nat. [ar \<mapsto> tsMap Bool\<cdot>(fst (tsRec\<cdot>(tsMap invBoolPair\<cdot>(Y i  .  dr)))), abpOut \<mapsto>
-                           tsMap Data\<cdot>(snd (tsRec\<cdot>(tsMap invBoolPair\<cdot>(Y i  .  dr))))]\<Omega>)"
+   show " c \<in> tsbDom\<cdot>(\<Squnion>i::nat. 
+                          [ar \<mapsto> tsMap Bool\<cdot>(fst (tsRec\<cdot>(tsMap invBoolPair\<cdot>(Y i  .  dr)))), 
+                       abpOut \<mapsto> tsMap Data\<cdot>(snd (tsRec\<cdot>(tsMap invBoolPair\<cdot>(Y i  .  dr))))]\<Omega>)"
      using assms(3) recv_tsb_dom tb_chain tsbChain_dom_eq2 by blast
 qed
    
      
 
   
-lemma recvTSPF_cont: "cont (\<lambda> x. (tsbDom\<cdot>x = {dr}) \<leadsto> [ar \<mapsto> tsMap Bool\<cdot>(fst (tsRec\<cdot>((tsMap invBoolPair)\<cdot>(x . dr)))),
-                                        abpOut \<mapsto> tsMap Data\<cdot>(snd (tsRec\<cdot>((tsMap invBoolPair)\<cdot>(x . dr))))]\<Omega>)"
+lemma recvTSPF_cont: 
+  shows "cont (\<lambda> x. (tsbDom\<cdot>x = {dr}) \<leadsto> 
+                      [ar \<mapsto> (tsMap::(bool \<Rightarrow> 'a MABP) \<Rightarrow> bool tstream \<rightarrow> 'a MABP tstream) 
+                            Bool\<cdot>(fst ((tsRec::('a * bool) tstream \<rightarrow> (bool tstream \<times> 'a tstream))\<cdot>
+                            ((tsMap invBoolPair)\<cdot>(x . dr)))),
+                       abpOut \<mapsto> (tsMap::('a \<Rightarrow> 'a MABP) \<Rightarrow> 'a tstream \<rightarrow> 'a MABP tstream) 
+                            Data\<cdot>(snd (tsRec\<cdot>((tsMap invBoolPair)\<cdot>(x . dr))))]\<Omega>)"
   proof (rule tspf_contI)
   
     show recv_mono: "\<And>(x::'a MABP TSB) y::'a MABP TSB. tsbDom\<cdot>x = {dr} \<Longrightarrow> x \<sqsubseteq> y \<Longrightarrow> 
@@ -217,26 +229,41 @@ lemma recvTSPF_cont: "cont (\<lambda> x. (tsbDom\<cdot>x = {dr}) \<leadsto> [ar 
       fix Y :: "nat \<Rightarrow> 'a MABP TSB"
       assume a1: "chain Y"
       assume a2: "tsbDom\<cdot>(\<Squnion>i. Y i) = {dr}"
-      have f3: "\<forall>t ta. (tsbDom\<cdot>t \<noteq> {dr} \<or> t \<notsqsubseteq> ta) \<or> [ar \<mapsto> tsMap Bool\<cdot> (fst (tsRec\<cdot>(tsMap invBoolPair\<cdot>(t . dr)))), abpOut \<mapsto> tsMap Data\<cdot> (snd (tsRec\<cdot> (tsMap invBoolPair\<cdot> (t . dr)))::'a tstream)]\<Omega> \<sqsubseteq> [ar \<mapsto> tsMap Bool\<cdot> (fst (tsRec\<cdot>(tsMap invBoolPair\<cdot>(ta . dr)))), abpOut \<mapsto> tsMap Data\<cdot> (snd (tsRec\<cdot>(tsMap invBoolPair\<cdot>(ta . dr))))]\<Omega>"
+      have f3: "\<forall>t ta. (tsbDom\<cdot>t \<noteq> {dr} \<or> t \<notsqsubseteq> ta) 
+                        \<or> [ar \<mapsto> tsMap Bool\<cdot> (fst (tsRec\<cdot>(tsMap invBoolPair\<cdot>(t . dr)))), 
+                            abpOut \<mapsto> tsMap Data\<cdot> (snd (tsRec\<cdot> (tsMap invBoolPair\<cdot> (t . dr)))::'a tstream)]\<Omega> 
+                          \<sqsubseteq> [ar \<mapsto> tsMap Bool\<cdot> (fst (tsRec\<cdot>(tsMap invBoolPair\<cdot>(ta . dr)))), 
+                              abpOut \<mapsto> tsMap Data\<cdot> (snd (tsRec\<cdot>(tsMap invBoolPair\<cdot>(ta . dr))))]\<Omega>"
         using recv_mono by blast
       have f4: "\<forall>f n. \<not> chain f \<or> tsbDom\<cdot>(f n::'a MABP TSB) = tsbDom\<cdot>(Lub f)"
         by (meson tsbChain_dom_eq2)
-      have f5: "\<And> elem_1 .tsbDom\<cdot> ([ar \<mapsto> tsMap Bool\<cdot> (fst (tsRec\<cdot>(tsMap invBoolPair\<cdot>(Y elem_1 . dr)))), abpOut \<mapsto> tsMap Data\<cdot> (snd (tsRec\<cdot> (tsMap invBoolPair\<cdot>(Y elem_1 . dr))))]\<Omega>) = {ar, abpOut}"
+      have f5: "\<And> elem_1 .tsbDom\<cdot> ([ar \<mapsto> tsMap Bool\<cdot> (fst (tsRec\<cdot>(tsMap invBoolPair\<cdot>(Y elem_1 . dr))))
+                          , abpOut \<mapsto> tsMap Data\<cdot> (snd (tsRec\<cdot> (tsMap invBoolPair\<cdot>(Y elem_1 . dr))))]\<Omega>) 
+                          = {ar, abpOut}"
         by (simp add: recv_tsb_dom)
-      have "\<And> v1_0. tsbDom\<cdot> (Y (v1_0 (\<lambda>n. [ar \<mapsto> tsMap Bool\<cdot> (fst (tsRec\<cdot>(tsMap invBoolPair\<cdot>(Y n . dr)))), abpOut \<mapsto> tsMap Data\<cdot> (snd (tsRec\<cdot> (tsMap invBoolPair\<cdot>(Y n . dr))))]\<Omega>))) = {dr}"
+      have "\<And> v1_0. tsbDom\<cdot> (Y (v1_0 (\<lambda>n. [ar \<mapsto> tsMap Bool\<cdot> (fst (tsRec\<cdot>(tsMap invBoolPair\<cdot>(Y n . dr)))), 
+                                           abpOut \<mapsto> tsMap Data\<cdot> (snd (tsRec\<cdot> (tsMap invBoolPair\<cdot>(Y n . dr))))]\<Omega>))) = {dr}"
         using f4 a2 a1 by presburger
-      then have "chain (\<lambda>n. [ar \<mapsto> tsMap Bool\<cdot> (fst (tsRec\<cdot>(tsMap invBoolPair\<cdot>(Y n . dr)))), abpOut \<mapsto> tsMap Data\<cdot> (snd (tsRec\<cdot>(tsMap invBoolPair\<cdot>(Y n . dr))))]\<Omega>)"
+      then have "chain (\<lambda>n. [ar \<mapsto> tsMap Bool\<cdot> (fst (tsRec\<cdot>(tsMap invBoolPair\<cdot>(Y n . dr)))), 
+                             abpOut \<mapsto> tsMap Data\<cdot> (snd (tsRec\<cdot>(tsMap invBoolPair\<cdot>(Y n . dr))))]\<Omega>)"
         using f3 a1 by (simp add: po_class.chain_def)
-      then show "tsbDom\<cdot> (\<Squnion>n. [ar \<mapsto> tsMap Bool\<cdot> (fst (tsRec\<cdot>(tsMap invBoolPair\<cdot>(Y n . dr)))), abpOut \<mapsto> tsMap Data\<cdot> (snd (tsRec\<cdot>(tsMap invBoolPair\<cdot>(Y n . dr))))]\<Omega>) = {abpOut, ar}"
+      then show "tsbDom\<cdot> (\<Squnion>n. [ar \<mapsto> tsMap Bool\<cdot> (fst (tsRec\<cdot>(tsMap invBoolPair\<cdot>(Y n . dr)))), 
+                               abpOut \<mapsto> tsMap Data\<cdot> (snd (tsRec\<cdot>(tsMap invBoolPair\<cdot>(Y n . dr))))]\<Omega>) = {abpOut, ar}"
         using f5 f4 by blast
     qed
       
-    (* maybe has to do with fixation and the type of the receiver *)
-   have f3: "\<And>(Y::nat \<Rightarrow> 'a MABP TSB) c::channel. chain Y \<Longrightarrow> tsbDom\<cdot>(\<Squnion>i::nat. Y i) = {dr} \<Longrightarrow> c = ar \<or> c = abpOut \<Longrightarrow> c = ar \<longrightarrow> tsMap Bool\<cdot>(fst (tsRec\<cdot>(tsMap invBoolPair\<cdot>(Lub Y  .  dr)))) \<sqsubseteq> (\<Squnion>i::nat. tsMap Bool\<cdot>(fst (tsRec\<cdot>(tsMap invBoolPair\<cdot>(Y i  .  dr)))))"
-     sorry
+      
+    have f3: "\<And>(Y::nat \<Rightarrow> 'a MABP TSB) c::channel. chain Y \<Longrightarrow> tsbDom\<cdot>(\<Squnion>i::nat. Y i) = {dr} 
+              \<Longrightarrow> c = ar \<or> c = abpOut \<Longrightarrow> c = ar \<longrightarrow> 
+              (tsMap::(bool \<Rightarrow> 'a MABP) \<Rightarrow> bool tstream \<rightarrow> 'a MABP tstream) Bool\<cdot>(fst (tsRec\<cdot>(tsMap invBoolPair\<cdot>(Lub Y  .  dr)))) 
+              \<sqsubseteq> (\<Squnion>i::nat. tsMap Bool\<cdot>(fst (tsRec\<cdot>(tsMap invBoolPair\<cdot>(Y i  .  dr)))))"
+     by (simp add: recvCH1_contlub to_recvch1)
        
-   have f4: "\<And>(Y::nat \<Rightarrow> 'a MABP TSB) c::channel. chain Y \<Longrightarrow> tsbDom\<cdot>(\<Squnion>i::nat. Y i) = {dr} \<Longrightarrow> c = ar \<or> c = abpOut \<Longrightarrow> c = ar \<longrightarrow>  tsMap Data\<cdot>(snd (tsRec\<cdot>(tsMap invBoolPair\<cdot>(Lub Y  .  dr)))) \<sqsubseteq> (\<Squnion>i::nat. tsMap Data\<cdot>(snd (tsRec\<cdot>(tsMap invBoolPair\<cdot>(Y i  .  dr)))))"
-     sorry
+   have f4: "\<And>(Y::nat \<Rightarrow> 'a MABP TSB) c::channel. chain Y \<Longrightarrow> tsbDom\<cdot>(\<Squnion>i::nat. Y i) = {dr} 
+               \<Longrightarrow> c = ar \<or> c = abpOut \<Longrightarrow> c = ar \<longrightarrow>  
+              tsMap Data\<cdot>(snd (tsRec\<cdot>(tsMap invBoolPair\<cdot>(Lub Y  .  dr)))) 
+               \<sqsubseteq> (\<Squnion>i::nat. tsMap Data\<cdot>(snd (tsRec\<cdot>(tsMap invBoolPair\<cdot>(Y i  .  dr)))))"
+    by (simp add: recvCH2_contlub to_recvch2)
        
     show "\<And>Y::nat \<Rightarrow> 'a MABP TSB.
        chain Y \<Longrightarrow>
